src/cbor/CBOR.Spec.Raw.fst
@@ -1,0 +1,84 @@
+module CBOR.Spec.Raw
+
+let rec raw_equiv (l1 l2: raw_data_item) : Tot bool (decreases l1) =
+  match l1, l2 with
+  | Simple v1, Simple v2 -> v1 = v2
+  | Int64 ty1 v1, Int64 ty2 v2 -> ty1 = ty2 && raw_uint64_equiv v1 v2
+  | String ty1 len1 v1, String ty2 len2 v2 -> ty1 = ty2 && raw_uint64_equiv len1 len2 && v1 = v2
+  | Array len1 v1, Array len2 v2 -> raw_uint64_equiv len1 len2 && wf_list_for_all2 v1 v2 raw_equiv
+  | Map len1 v1, Map len2 v2 ->
+    raw_uint64_equiv len1 len2 &&
+    wf_list_for_all_exists v1 v2 raw_pair_equiv &&
+    wf_list_for_all_exists v2 v1 raw_pair_equiv_swap
+  | Tagged tag1 v1, Tagged tag2 v2 ->
+    raw_uint64_equiv tag1 tag2 &&
+    raw_equiv v1 v2
+  | _ -> false
+
+and raw_pair_equiv (l1 l2: (raw_data_item & raw_data_item)) : Tot bool (decreases l1) =
+  raw_equiv (fst l1) (fst l2) && raw_equiv (snd l1) (snd l2)
+
+and raw_pair_equiv_swap (l2 l1: (raw_data_item & raw_data_item)) : Tot bool (decreases l1) =
+  raw_equiv (fst l1) (fst l2) && raw_equiv (snd l1) (snd l2)
+
+let rec raw_equiv_eq' (l1 l2: raw_data_item) : Lemma (ensures
+  raw_equiv l1 l2 == begin match l1, l2 with
+  | Simple v1, Simple v2 -> v1 = v2
+  | Int64 ty1 v1, Int64 ty2 v2 -> ty1 = ty2 && raw_uint64_equiv v1 v2
+  | String ty1 len1 v1, String ty2 len2 v2 -> ty1 = ty2 && raw_uint64_equiv len1 len2 && v1 = v2
+  | Array len1 v1, Array len2 v2 -> raw_uint64_equiv len1 len2 && list_for_all2 raw_equiv v1 v2
+  | Map len1 v1, Map len2 v2 ->
+    raw_uint64_equiv len1 len2 &&
+    list_for_all_exists (holds_on_pair2 raw_equiv) v1 v2 &&
+    list_for_all_exists (holds_on_pair2 raw_equiv) v2 v1
+  | Tagged tag1 v1, Tagged tag2 v2 ->
+    raw_uint64_equiv tag1 tag2 &&
+    raw_equiv v1 v2
+  | _ -> false
+  end /\
+  (raw_equiv l1 l2 == raw_equiv l2 l1)
+)
+(decreases l1)
+= match l1, l2 with
+  | Array len1 v1, Array len2 v2 ->
+    assert_norm (raw_equiv (Array len1 v1) (Array len2 v2) == (raw_uint64_equiv len1 len2 && wf_list_for_all2 v1 v2 raw_equiv));
+    assert_norm (raw_equiv (Array len2 v2) (Array len1 v1) == (raw_uint64_equiv len2 len1 && wf_list_for_all2 v2 v1 raw_equiv));
+    wf_list_for_all2_eq raw_equiv v1 v2;
+    wf_list_for_all2_eq raw_equiv v2 v1;
+    list_for_all2_ext raw_equiv (swap raw_equiv) v1 v2 (fun x1 x2 ->
+      raw_equiv_eq' x1 x2
+    );
+    list_for_all2_swap raw_equiv v2 v1;
+    assert (list_for_all2 raw_equiv v1 v2 == list_for_all2 raw_equiv v2 v1)
+  | Map len1 v1, Map len2 v2 ->
+    assert_norm (raw_equiv (Map len1 v1) (Map len2 v2) == (
+      raw_uint64_equiv len1 len2 &&
+      wf_list_for_all_exists v1 v2 raw_pair_equiv &&
+      wf_list_for_all_exists v2 v1 raw_pair_equiv_swap
+    ));
+    assert_norm (raw_equiv (Map len2 v2) (Map len1 v1) == (
+      raw_uint64_equiv len2 len1 &&
+      wf_list_for_all_exists v2 v1 raw_pair_equiv &&
+      wf_list_for_all_exists v1 v2 raw_pair_equiv_swap
+    ));
+    wf_list_for_all_exists_eq raw_pair_equiv v1 v2;
+    list_for_all_exists_ext raw_pair_equiv (holds_on_pair2 raw_equiv) v1 v2 (fun _ _ -> ());
+    wf_list_for_all_exists_eq raw_pair_equiv_swap v2 v1;
+    list_for_all_exists_ext raw_pair_equiv_swap (holds_on_pair2 raw_equiv) v2 v1 (fun x2 x1 ->
+      raw_equiv_eq' (fst x1) (fst x2);
+      raw_equiv_eq' (snd x1) (snd x2)
+    );
+    wf_list_for_all_exists_eq raw_pair_equiv v2 v1;
+    list_for_all_exists_ext raw_pair_equiv (holds_on_pair2 raw_equiv) v2 v1 (fun _ _ -> ());
+    wf_list_for_all_exists_eq raw_pair_equiv_swap v1 v2;
+    list_for_all_exists_ext raw_pair_equiv_swap (holds_on_pair2 raw_equiv) v1 v2 (fun x1 x2 ->
+      raw_equiv_eq' (fst x1) (fst x2);
+      raw_equiv_eq' (snd x1) (snd x2)
+    )
+  | Tagged tag1 v1, Tagged tag2 v2 ->
+    raw_equiv_eq' v1 v2
+  | _ -> ()
+
+let raw_equiv_eq l1 l2 = raw_equiv_eq' l1 l2
+
+let raw_equiv_sym l1 l2 = raw_equiv_eq' l1 l2
